pulse/src/syntax_extension/PulseSyntaxExtension.Sugar.fst
@@ -17,6 +17,7 @@
 module PulseSyntaxExtension.Sugar
 open FStar.Ident
 module A = FStar.Parser.AST
+module AU = FStar.Parser.AST.Util
 let rng = FStar.Compiler.Range.range
 let dummyRange = FStar.Compiler.Range.dummyRange
 
@@ -215,6 +216,155 @@ let tag_of_stmt (s:stmt) : string =
 type decl =
   | FnDefn of fn_defn
   | FnDecl of fn_decl
+open FStar.Class.Deq
+let eq_ident (i1 i2:Ident.ident) = i1 =? i2
+let eq_lident (i1 i2:Ident.lident) = i1 =? i2
+let rec forall2 (f:'a -> 'a -> bool) (l1 l2:list 'a) : bool =
+  match l1, l2 with
+  | [], [] -> true
+  | x::xs, y::ys -> f x y && forall2 f xs ys
+  | _, _ -> false
+let eq_opt (eq:'a -> 'a -> bool) (o1:option 'a) (o2:option 'a) =
+  match o1, o2 with
+  | Some x, Some y -> eq x y
+  | None, None -> true
+  | _, _ -> false
+let rec eq_decl (d1 d2:decl) =
+  match d1, d2 with
+  | FnDefn f1, FnDefn f2 -> eq_fn_defn f1 f2
+  | FnDecl d1, FnDecl d2 -> eq_fn_decl d1 d2
+and eq_fn_decl (f1 f2:fn_decl) =
+  eq_ident f1.id f2.id &&
+  forall2 AU.eq_binder f1.binders f2.binders &&
+  eq_ascription f1.ascription f2.ascription
+and eq_fn_defn (f1 f2:fn_defn) =
+  eq_ident f1.id f2.id &&
+  f1.is_rec = f2.is_rec &&
+  forall2 AU.eq_binder f1.binders f2.binders &&
+  eq_ascription f1.ascription f2.ascription &&
+  eq_opt AU.eq_term f1.measure f2.measure &&
+  eq_body f1.body f2.body
+and eq_ascription (a1 a2:either computation_type (option A.term)) =
+  match a1, a2 with
+  | Inl c1, Inl c2 -> eq_computation_type c1 c2
+  | Inr t1, Inr t2 -> eq_opt AU.eq_term t1 t2
+  | _, _ -> false
+and eq_computation_type (c1 c2:computation_type) =
+  c1.tag = c2.tag &&
+  eq_slprop c1.precondition c2.precondition &&
+  eq_ident c1.return_name c2.return_name &&
+  AU.eq_term c1.return_type c2.return_type &&
+  eq_slprop c1.postcondition c2.postcondition &&
+  eq_opt AU.eq_term c1.opens c2.opens
+and eq_slprop (s1 s2:slprop) =
+  eq_slprop' s1.v s2.v
+and eq_slprop' (s1 s2:slprop') =
+  match s1, s2 with
+  | SLPropTerm t1, SLPropTerm t2 -> AU.eq_term t1 t2
+and eq_body (b1 b2:either stmt lambda) =
+  match b1, b2 with
+  | Inl s1, Inl s2 -> eq_stmt s1 s2
+  | Inr l1, Inr l2 -> eq_lambda l1 l2
+  | _, _ -> false
+and eq_stmt (s1 s2:stmt) =
+  eq_stmt' s1.s s2.s
+and eq_stmt' (s1 s2:stmt') =
+  match s1, s2 with
+  | Open l1, Open l2 -> eq_lident l1 l2
+  | Expr e1, Expr e2 -> AU.eq_term e1.e e2.e
+  | Assignment { lhs=l1; value=v1 }, Assignment { lhs=l2; value=v2 } ->
+    AU.eq_term l1 l2 && AU.eq_term v1 v2
+  | ArrayAssignment { arr=a1; index=i1; value=v1 }, ArrayAssignment { arr=a2; index=i2; value=v2 } ->
+    AU.eq_term a1 a2 && AU.eq_term i1 i2 && AU.eq_term v1 v2
+  | LetBinding { qualifier=q1; id=i1; typ=t1; init=init1 }, LetBinding { qualifier=q2; id=i2; typ=t2; init=init2 } ->
+    eq_opt eq_mut_or_ref q1 q2 &&
+    eq_ident i1 i2 &&
+    eq_opt AU.eq_term t1 t2 &&
+    eq_opt eq_let_init init1 init2
+  | Block { stmt=s1 }, Block { stmt=s2 } -> eq_stmt s1 s2
+  | If { head=h1; join_slprop=j1; then_=t1; else_opt=e1 }, If { head=h2; join_slprop=j2; then_=t2; else_opt=e2 } ->
+    AU.eq_term h1 h2 &&
+    eq_opt eq_ensures_slprop j1 j2 &&
+    eq_stmt t1 t2 &&
+    eq_opt eq_stmt e1 e2
+  | Match { head=h1; returns_annot=r1; branches=b1 }, Match { head=h2; returns_annot=r2; branches=b2 } ->
+    AU.eq_term h1 h2 &&
+    eq_opt eq_ensures_slprop r1 r2 &&
+    forall2 (fun (p1, s1) (p2, s2) -> AU.eq_pattern p1 p2 && eq_stmt s1 s2) b1 b2
+  | While { guard=g1; id=id1; invariant=i1; body=b1 }, While { guard=g2; id=id2; invariant=i2; body=b2 } ->
+    eq_stmt g1 g2 &&
+    eq_ident id1 id2 &&
+    eq_slprop i1 i2 &&
+    eq_stmt b1 b2
+  | Introduce { slprop=s1; witnesses=w1 }, Introduce { slprop=s2; witnesses=w2 } ->
+    eq_slprop s1 s2 &&
+    forall2 AU.eq_term w1 w2
+  | Sequence { s1=s1; s2=s2 }, Sequence { s1=s1'; s2=s2' } ->
+    eq_stmt s1 s1' && eq_stmt s2 s2'
+  | Parallel { p1=p1; p2=p2; q1=q1; q2=q2; b1=b1; b2=b2 }, Parallel { p1=p1'; p2=p2'; q1=q1'; q2=q2'; b1=b1'; b2=b2' } ->
+    eq_slprop p1 p1' &&
+    eq_slprop p2 p2' &&
+    eq_slprop q1 q1' &&
+    eq_slprop q2 q2' &&
+    eq_stmt b1 b1' &&
+    eq_stmt b2 b2'
+  | ProofHintWithBinders { hint_type=ht1; binders=bs1 }, ProofHintWithBinders { hint_type=ht2; binders=bs2 } ->
+    eq_hint_type ht1 ht2 &&
+    forall2 AU.eq_binder bs1 bs2
+  | WithInvariants { names=n1; body=b1; returns_=r1 }, WithInvariants { names=n2; body=b2; returns_=r2 } ->
+    forall2 AU.eq_term n1 n2 &&
+    eq_stmt b1 b2 &&
+    eq_opt eq_ensures_slprop r1 r2
+and eq_let_init (i1 i2:let_init) =
+  match i1, i2 with
+  | Array_initializer a1, Array_initializer a2 -> eq_array_init a1 a2
+  | Default_initializer t1, Default_initializer t2 -> AU.eq_term t1 t2
+  | Lambda_initializer l1, Lambda_initializer l2 -> eq_fn_defn l1 l2
+  | Stmt_initializer s1, Stmt_initializer s2 -> eq_stmt s1 s2
+  | _, _ -> false
+and eq_array_init (a1 a2:array_init) =
+  AU.eq_term a1.init a2.init && AU.eq_term a1.len a2.len
+and eq_hint_type (h1 h2:hint_type) =
+  match h1, h2 with
+  | ASSERT s1, ASSERT s2 -> eq_slprop s1 s2
+  | UNFOLD (ns1, s1), UNFOLD (ns2, s2) ->
+    eq_opt (forall2 eq_lident) ns1 ns2 &&
+    eq_slprop s1 s2
+  | FOLD (ns1, s1), FOLD (ns2, s2) ->
+    eq_opt (forall2 eq_lident) ns1 ns2 &&
+    eq_slprop s1 s2
+  | RENAME (ts1, g1, t1), RENAME (ts2, g2, t2) ->
+    forall2 (fun (t1, t2) (t1', t2') -> AU.eq_term t1 t1' && AU.eq_term t2 t2') ts1 ts2 &&
+    eq_opt eq_slprop g1 g2 &&
+    eq_opt AU.eq_term t1 t2
+  | REWRITE (s1, s1', t1), REWRITE (s2, s2', t2) ->
+    eq_slprop s1 s2 &&
+    eq_slprop s1' s2' &&
+    eq_opt AU.eq_term t1 t2
+  | WILD, WILD -> true
+  | SHOW_PROOF_STATE r1, SHOW_PROOF_STATE r2 -> true
+  | _, _ -> false
+and eq_ensures_slprop (e1 e2:ensures_slprop) =
+  let h1, s1, t1 = e1 in
+  let h2, s2, t2 = e2 in
+  eq_opt (fun (i1, t1) (i2, t2) -> eq_ident i1 i2 && AU.eq_term t1 t2) h1 h2 &&
+  eq_slprop s1 s2 &&
+  eq_opt AU.eq_term t1 t2
+and eq_lambda (l1 l2:lambda) =
+  forall2 AU.eq_binder l1.binders l2.binders &&
+  eq_opt eq_computation_type l1.ascription l2.ascription &&
+  eq_stmt l1.body l2.body
+and eq_mut_or_ref (m1 m2:mut_or_ref) =
+  match m1, m2 with
+  | MUT, MUT -> true
+  | REF, REF -> true
+  | _, _ -> false
+and eq_pat (p1 p2:pat) =
+  match p1, p2 with
+  | PatVar i1, PatVar i2 -> eq_ident i1 i2
+  | PatConstructor { head=h1; args=a1 }, PatConstructor { head=h2; args=a2 } ->
+    eq_lident h1 h2 && forall2 eq_pat a1 a2
+  | _, _ -> false
 
 let range_of_decl (d:decl) =
   match d with
