pulse/src/syntax_extension/PulseSyntaxExtension.ASTBuilder.fst
@@ -158,7 +158,15 @@ let parse_extension_lang (contents:string) (r:FStar.Compiler.Range.range)
       : decl
       = let id, r = id_and_range_of_decl d in  
         let id_txt = Ident.string_of_id id in
-        let decl_as_term = tm (DesugaredBlob <| FStar.Syntax.Util.mk_lazy d S.t_bool (S.Lazy_extension "pulse_sugar_decl") (Some r)) r in
+        let decl_as_term = 
+          let blob = FStar.Syntax.Util.mk_lazy d S.t_bool (S.Lazy_extension "pulse_sugar_decl") (Some r) in
+          let eq (t1 t2: FStar.Syntax.Syntax.term) =
+             let d1 : PulseSyntaxExtension.Sugar.decl = FStar.Syntax.Util.unlazy_as_t (S.Lazy_extension "pulse_sugar_decl") t1 in
+             let d2 : PulseSyntaxExtension.Sugar.decl = FStar.Syntax.Util.unlazy_as_t (S.Lazy_extension "pulse_sugar_decl") t2 in
+             PulseSyntaxExtension.Sugar.eq_decl d1 d2
+          in
+          tm (DesugaredBlob {tag="pulse_sugar_decl"; blob; eq}) r
+        in
         let splicer =
           let head = tm (Var pulse_checker_after_parse_tac) r in
           let namespaces, abbrevs = encode_open_namespaces_and_abbreviations ctx r in
